todos for the next week

theories/examples/run_yield_1_adequacy.v
@@ -38,21 +38,7 @@ Section Adequacy.
                                   (mem_layout σ p1 p2) ∧
                                   (reg σ p1 p2) ∧
                                   transactions σ.
-
-  (*
-  Definition reg_final (σ : state) (p1 : PID) :=
-    let gm : gmap reg_name handle := {[ PC := ((of_pid p1) ^+ (length program1))%f; R0 := yield_I; R1 := (encode_vmid V1) ]} in
-    gm ⊆ ((get_reg_files σ) !!! V0).
-
-  Definition is_final_config (σ : state) (ms : list exec_mode) (φs : list (exec_mode -> Prop)) :=
-    (get_current_vm σ) = V0 ∧
-    φs = [(λ m , m = HaltI); (λ _, False)] ∧
-    ∃ (p1 p2: PID), p1 ≠ p2 ∧
-                    (run_vms ms) ∧
-                    (mem_layout σ p1 p2) ∧
-                    (reg_final σ p1) ∧
-                    transactions σ.
-   *)
+  
   Definition irisΣ :=
     #[gen_VMΣ; invΣ; na_invΣ; savedPropΣ; GFunctor (authUR (optionUR (frac_agreeR gnameO)));
      GFunctor (authUR (gmapUR nat (agreeR gnameO)))].
@@ -66,7 +52,7 @@ Section Adequacy.
   Context {vm_preG: gen_VMPreG Addr VMID Word reg_name PID transaction_type irisΣ}.
 
   (* exec_mode of all VMs *)
-  Lemma run_yield_1_adequacy' (σ : state) (ms : list exec_mode) φs:
+  Lemma run_yield_1_adequacy (σ : state) (ms : list exec_mode) φs:
     (* we need assumptions to be able to allocate resources *)
     (* with these resources, we apply the specification and get the wptp *)
     (* along with some other stuff, then it should be enough to apply the adequacy theorem *)
@@ -437,4 +423,404 @@ Section Adequacy.
     iFrame.    
   Qed.
 
+  Definition reg_final (σ : state) (p1 p2 : PID) :=
+    let gm0 := {[ PC := ((of_pid p1) ^+ (length program1))%f; R0 := of_imm yield_I; R1 := of_imm (encode_vmid V1) ]} in
+    let gm1 := {[ PC := ((of_pid p2) ^+ (length program2))%f; R0 := of_imm yield_I ]} in
+    (gm0 ⊆ ((get_reg_files σ) !!! V0)) ∧ (gm1 ⊆ ((get_reg_files σ) !!! V1)).
+
+  Definition is_final_config (σ: state) :=
+                  (get_current_vm σ) = V0 ∧
+                  ∃ (p1 p2: PID), p1 ≠ p2 ∧
+                                  (reg_final σ p1 p2).
+
+  Definition is_initial_config' (σ: state) :=
+    (get_current_vm σ) = V0 ∧    
+    ∃ (p1 p2: PID), p1 ≠ p2 ∧
+                    (mem_layout σ p1 p2) ∧
+                    (reg σ p1 p2) ∧
+                    transactions σ.
+
+  (* TODO: we need an invariant here *)
+  Lemma run_yield_1_adequacy' (σ σ' : state) :
+    (is_initial_config' σ) ->
+    rtc machine.step ([ExecI; ExecI], σ) ([HaltI; ExecI], σ') →
+    True (*(is_final_config σ')*).
+  Proof.
+    intros Hinit.
+    set (saved_props := (let (_, x, _, _) := iris_subG irisΣ (subG_refl irisΣ) in x)).
+    set (prop_name := (let (_, _, x, _) := iris_subG irisΣ (subG_refl irisΣ) in x)).
+    set (name_map := (let (_, _, _, x) := iris_subG irisΣ (subG_refl irisΣ) in x)).
+    eapply (wp_invariance irisΣ); auto.
+    destruct Hinit as (Hcur & (p1 & p2 & p1p2ne & Hmem & Hreg & Htrans)).
+    intro Hinv.
+    iStartProof.
+    iMod (gen_mem_alloc (get_mem σ)) as (mem_gname) "[Hσmem Hmem]".
+    iMod (gen_reg_alloc (get_reg_gmap σ)) as (reg_gname) "[Hσreg Hreg]".
+    iMod (gen_tx_alloc (get_tx_agree σ)) as (tx_gname) "[Hσtx _]".
+    { apply get_txrx_auth_agree_valid. }
+    iMod (gen_rx_agree_alloc (get_rx_agree σ)) as (rx_agree_gname) "[Hσrx_a _]".
+    { apply get_txrx_auth_agree_valid. }
+    iMod (gen_rx_option_alloc (get_rx_gmap σ)) as (rx_option_gname) "[Hσrx_o _]".
+    iMod (gen_pagetable_alloc (get_owned_gmap σ)) as (own_gname) "[Hσown _]".
+    iMod (gen_pagetable_alloc (get_access_gmap σ)) as (access_gname) "[Hσaccess Haccess]".
+    iMod (gen_pagetable_alloc (get_excl_gmap σ)) as (excl_gname) "[Hσexcl _]".
+    iMod (gen_trans_alloc (get_trans_gmap σ)) as (trans_gname) "[Hσtrans _]".
+    iMod (gen_hpool_alloc (get_hpool_gset σ)) as (hpool_gname) "[Hσhpool _]".
+    iMod (gen_retri_alloc (get_retri_gmap σ)) as (retri_gname) "[Hσretri _]".
+    iMod (na_alloc) as (nainv_gname) "Hna".
+
+    iModIntro.
+    iIntros (name_map_name).
+    pose ((GenVMG irisΣ vm_preG Hinv _ nainv_gname _ _ _ name_map_name mem_gname reg_gname tx_gname rx_agree_gname rx_option_gname own_gname access_gname excl_gname trans_gname hpool_gname retri_gname)) as VMG.
+    iExists (gen_vm_interp (Σ := irisΣ)).
+
+    iModIntro.
+
+    iExists [True%I; ((R0 @@ V0 ->r run_I ∗ R1 @@ V0 ->r encode_vmid V1) ∗ VMProp V0 ((R0 @@ V0 ->r yield_I ∗ R1 @@ V0 ->r encode_vmid V1) ∗ VMProp V1 False%I (1/2)%Qp) (1/2)%Qp)%I].
+    iSimpl.
+    iSplit; first done.
+
+    destruct Hreg as (Hreg1 & Hreg2).
+    destruct Hreg1 as (r0_ & r1_ & Hreg1).
+    destruct Hreg2 as (r0_' & Hreg2).
+    destruct Htrans as (Hdisj & Hnempty & Hlen).
+
+    iSplitR "Hmem Hreg Haccess Hna".
+    iFrame.
+    assert (vm_count = 2) as ->.
+    unfold vm_count.
+    unfold vmconfig.
+    done.
+    iSplit; first done.
+    iSplit; first done.
+    done.   
+    
+    iDestruct ((big_sepM_subseteq _ (get_reg_gmap σ) {[(PC, V0):= (of_pid p1); (R0, V0) := r0_;
+                                 (R1,V0):= r1_ ; (PC,V1):= (of_pid p2); (R0,V1):= r0_' ]}) with "Hreg") as "Hreg";eauto.
+    { rewrite /get_reg_gmap.
+      apply map_subseteq_spec.
+      intros i x H.
+      rewrite /flat_map.
+      simpl.
+      apply elem_of_list_to_map_1'.
+      intros y P.
+      apply elem_of_list_In in P.
+      rewrite ->!in_app_iff in P.
+      destruct P as [P | [P | P]].
+      - apply in_map_iff in P.
+        destruct P as [[a b] [PEq P]].
+        simpl in PEq.
+        destruct i as [i1 i2].
+        inversion PEq.
+        subst.        
+        clear PEq.
+        rewrite <-elem_of_list_In in P.
+        apply elem_of_map_to_list' in P.
+        simpl in P.
+        unfold get_vm_reg_file in *.
+        apply Some_eq_inj.
+        pose proof ((iffLR (map_subseteq_spec _ _)) Hreg1 i1 x) as HTemp1.
+        rewrite <-P.        
+        rewrite <-HTemp1.
+        unfold V0.
+        by simpl.
+        rewrite <-H.
+        destruct i1; simplify_map_eq /=.
+        + by rewrite lookup_insert.
+        + destruct n.
+          unfold R0 in *.
+          rewrite (@proof_irrel (0 < 31) (nat_lt_pi 0 31) machine_extra.R0_obligation_1 fin).
+          rewrite (@proof_irrel (0 < 31) (nat_lt_pi 0 31) machine_extra.R0_obligation_1 fin) in H.
+          unfold V0 in *.
+          simplify_map_eq /=.
+          rewrite lookup_insert_ne.
+          by rewrite lookup_insert.
+          discriminate.
+          destruct n.
+          unfold R1 in *.
+          rewrite (@proof_irrel (1 < 31) (nat_lt_pi 1 31) machine_extra.R1_obligation_1 fin).
+          rewrite (@proof_irrel (1 < 31) (nat_lt_pi 1 31) machine_extra.R1_obligation_1 fin) in H.
+          unfold V0 in *.
+          simplify_map_eq /=.
+          rewrite lookup_insert_ne.
+          rewrite lookup_insert_ne.
+          by rewrite lookup_insert.
+          discriminate.
+          discriminate.
+          simplify_map_eq /=.
+      - apply in_map_iff in P.
+        destruct P as [[a b] [PEq P]].
+        simpl in PEq.
+        destruct i as [i1 i2].
+        inversion PEq.
+        subst.        
+        clear PEq.
+        rewrite <-elem_of_list_In in P.
+        apply elem_of_map_to_list' in P.
+        simpl in P.
+        unfold get_vm_reg_file in *.
+        apply Some_eq_inj.
+        pose proof ((iffLR (map_subseteq_spec _ _)) Hreg2 i1 x) as HTemp1.
+        rewrite <-P.        
+        rewrite <-HTemp1.
+        unfold V1.
+        by simpl.
+        rewrite <-H.
+        destruct i1; simplify_map_eq /=.
+        + by rewrite lookup_insert.
+        + destruct n.
+          unfold R0 in *.
+          rewrite (@proof_irrel (0 < 31) (nat_lt_pi 0 31) machine_extra.R0_obligation_1 fin).
+          rewrite (@proof_irrel (0 < 31) (nat_lt_pi 0 31) machine_extra.R0_obligation_1 fin) in H.
+          unfold V1 in *.
+          simplify_map_eq /=.
+          rewrite lookup_insert_ne.
+          by rewrite lookup_insert.
+          discriminate.
+          destruct n.
+          unfold R0 in H.
+          inversion H.
+          discriminate.
+      - inversion P.
+      - rewrite app_nil_r.
+        apply elem_of_list_In.
+        rewrite in_app_iff.
+        rewrite !in_map_iff.
+        destruct i as [ir iv].
+        unfold VMID in iv.
+        unfold vm_count in iv.
+        cbn in iv.
+        dependent destruction iv.
+        + left.
+          exists (ir, x).
+          split; auto.
+          rewrite <-elem_of_list_In.
+          apply elem_of_map_to_list'.
+          simpl.
+          rewrite /get_vm_reg_file.
+          destruct ir; simplify_map_eq /=.
+          * unfold V0 in Hreg1.
+            simpl in Hreg1.
+            apply ((iffLR (map_subseteq_spec _ _)) Hreg1 PC p1).
+            by rewrite lookup_insert.
+          * destruct n.
+            unfold R0 in *.
+            simpl in *.
+            rewrite (@proof_irrel (0 < 31) (nat_lt_pi 0 31) machine_extra.R0_obligation_1 fin) in H.
+            rewrite (@proof_irrel (0 < 31) (nat_lt_pi 0 31) machine_extra.R0_obligation_1 fin) in Hreg1.
+            unfold V0 in Hreg1.
+            simpl in Hreg1.
+            simplify_map_eq /=.
+            apply ((iffLR (map_subseteq_spec _ _)) Hreg1 _ x).
+            rewrite lookup_insert_ne.
+            by rewrite lookup_insert.
+            discriminate.
+            destruct n.
+            unfold R1 in *.
+            simpl in *.
+            rewrite (@proof_irrel (1 < 31) (nat_lt_pi 1 31) machine_extra.R1_obligation_1 fin) in H.
+            rewrite (@proof_irrel (1 < 31) (nat_lt_pi 1 31) machine_extra.R1_obligation_1 fin) in Hreg1.
+            unfold V0 in Hreg1.
+            simpl in Hreg1.
+            simplify_map_eq /=.
+            apply ((iffLR (map_subseteq_spec _ _)) Hreg1 _ x).
+            rewrite lookup_insert_ne.
+            rewrite lookup_insert_ne.
+            by rewrite lookup_insert.
+            discriminate.
+            discriminate.
+            simplify_map_eq /=.
+        + right.
+          exists (ir, x).
+          split.
+          simpl.
+          repeat f_equal.
+          dependent destruction iv; auto.
+          inversion iv.
+          dependent destruction iv; auto.
+          2 : { inversion iv. }
+          rewrite <-elem_of_list_In.
+          apply elem_of_map_to_list'.
+          simpl.
+          rewrite /get_vm_reg_file.
+          destruct ir; simplify_map_eq /=.
+          * unfold V1 in Hreg2.
+            simpl in Hreg2.
+            apply ((iffLR (map_subseteq_spec _ _)) Hreg2 PC p2).
+            simplify_map_eq /=.
+            by rewrite lookup_insert.
+          * inversion H.
+            simplify_eq.
+            unfold R0 in *.
+            simpl in *.
+            rewrite (@proof_irrel (0 < 31) (nat_lt_pi 0 31) machine_extra.R0_obligation_1 fin) in H.
+            rewrite (@proof_irrel (0 < 31) (nat_lt_pi 0 31) machine_extra.R0_obligation_1 fin) in Hreg2.
+            unfold V1 in Hreg2.
+            simpl in Hreg2.
+            simplify_map_eq /=.
+            apply ((iffLR (map_subseteq_spec _ _)) Hreg2 _ x).
+            rewrite lookup_insert_ne.
+            by rewrite lookup_insert.
+            discriminate.
+    }
+    
+    iDestruct ((gen_pagetable_SepM_split2 V0 V1 (vmG := VMG) (σ := σ) (γ := access_gname) (λ pt, pt.2) is_accessible) with "[Haccess]") as "(Haccessz & Haccessi & _)"; eauto.
+    set (sacc1 := (get_pagetable_gset σ V0 (λ pt : page_table, pt.2) is_accessible)) in *.
+    set (sacc2 := (get_pagetable_gset σ V1 (λ pt : page_table, pt.2) is_accessible)) in *.    
+
+    rewrite !big_sepM_insert ?big_sepM_empty;eauto.
+    rewrite reg_mapsto_eq /reg_mapsto_def.
+    iDestruct "Hreg" as "(PCz & R0z & R1z & PCi & R0i & _)".
+    2: { rewrite !lookup_insert_None; split;eauto. }
+    2: { rewrite !lookup_insert_None; split;eauto. }
+    2: { rewrite !lookup_insert_None; split;eauto. }
+    2: { rewrite !lookup_insert_None; split;eauto. }
+
+    iDestruct ((big_sepM_subseteq _ (get_mem σ) (mk_region p1 program1 ∪ mk_region p2 program2))
+                 with "Hmem") as "Hmem"; eauto.
+    rewrite /mem_layout in Hmem.
+    by (destruct Hmem as (_ & _ & ?)).
+    
+    iDestruct ((big_sepM_union _ _) with "Hmem") as "[Hprog1 Hprog2]".
+    {
+      rewrite /mk_region.
+      apply map_disjoint_list_to_map_zip_r_2.
+      rewrite finz_seq_length //.
+      apply Forall_forall.
+      intros.
+      apply  not_elem_of_list_to_map_1.
+      rewrite fst_zip.
+      apply (addr_in_notin p2 p1 x (length program2));eauto.
+      by vm_compute.
+      by vm_compute.
+      rewrite finz_seq_length //.
+    }
+
+    destruct Hmem as (Hacc1 & Hacc2 & Hmem).
+    
+    pose proof (@run_yield_1_spec _ _ VMG 1 1 p1 p2 sacc1 sacc2)
+      as HSpec.
+
+    set (x := (@rules_base.hyp_irisG vmconfig hypparams irisΣ VMG)).
+    set (y := (IrisG (@hyp_machine vmconfig hypparams) irisΣ Hinv (@irisG_saved_prop irisΣ (iris_subG irisΣ (subG_refl irisΣ)))
+                (@irisG_prop_name irisΣ (iris_subG irisΣ (subG_refl irisΣ))) (@irisG_name_map irisΣ (iris_subG irisΣ (subG_refl irisΣ))) name_map_name
+                (@gen_vm_interp vmconfig irisΣ VMG))).
+    cbn in x.
+    cbn in y.
+
+    iSplitL "PCz R0z R1z PCi R0i Haccessz Haccessi Hprog1 Hprog2".
+    
+    iIntros "(VMProp0 & VMProp1 & _)".
+    rewrite /scheduled /machine.scheduler //= /scheduler Hcur //=.
+
+    iDestruct (HSpec with "[VMProp0 VMProp1 PCz PCi R0z R0i R1z Haccessz Haccessi Hprog1 Hprog2]") as "HWPs"; eauto.
+    {
+      rewrite /program1 //=.
+      unfold seq_in_page. split. solve_finz. split. unfold Is_true. case_match;[done|solve_finz].
+      split.
+      pose proof (last_addr_in_bound p1).
+      solve_finz.
+      unfold Is_true. case_match;[done|solve_finz].
+    }
+    { apply elem_of_list_to_set.
+      apply elem_of_list_In.
+      apply in_map_iff.
+      destruct Hacc1 as [a Hacc1].
+      exists (p1, a).
+      split;[done|].
+      apply elem_of_list_In.
+      apply elem_of_map_to_list.
+      apply map_filter_lookup_Some.
+      destruct Hacc1;split;done.
+    }
+    {
+      rewrite /program2 //=.
+      unfold seq_in_page. split. solve_finz. split. unfold Is_true. case_match;[done|solve_finz].
+      split.
+      pose proof (last_addr_in_bound p2).
+      solve_finz.
+      unfold Is_true. case_match;[done|solve_finz].
+    }
+    {
+      apply elem_of_list_to_set.
+      apply elem_of_list_In.
+      apply in_map_iff.
+      destruct Hacc2 as [a Hacc2].
+      exists (p2, a).
+      split;[done|].
+      apply elem_of_list_In.
+      apply elem_of_map_to_list.
+      apply map_filter_lookup_Some.
+      destruct Hacc2;split;done.
+    }
+    iSimpl.
+
+    {
+    rewrite /program.
+    iSplitL "Hprog1".
+    {
+    iApply (big_sepL2_alt with "[Hprog1]").
+    iSplitR.
+    rewrite finz_seq_length //.
+    rewrite <- (@map_to_list_to_map Addr (gmap Addr) _  _  _  _ _ _ _ _ _ Word _).
+    2: { rewrite fst_zip. apply finz_seq_NoDup'. pose proof (last_addr_in_bound p1). solve_finz.
+       rewrite finz_seq_length //. }
+    rewrite -(big_opM_map_to_list (λ a w,  (a ->a w)%I) _ ).
+    rewrite  mem_mapsto_eq /mem_mapsto_def /mk_region.
+    iFrame.
+    }
+
+    iSplitL "Hprog2".
+    iApply (big_sepL2_alt with "[Hprog2]").
+    iSplitR.
+    rewrite finz_seq_length //.
+    rewrite <- (@map_to_list_to_map Addr (gmap Addr) _  _  _  _ _ _ _ _ _ Word _).
+    2: { rewrite fst_zip. apply finz_seq_NoDup'. pose proof (last_addr_in_bound p2). solve_finz.
+       rewrite finz_seq_length //. }
+    rewrite -(big_opM_map_to_list (λ a w,  (a ->a w)%I) _ ).
+    rewrite  mem_mapsto_eq /mem_mapsto_def /mk_region.
+    iFrame.
+    rewrite reg_mapsto_eq /reg_mapsto_def.
+    rewrite access_mapsto_eq /access_mapsto_def.
+    rewrite /gen_access_name /gen_reg_name.
+    cbn.
+    iFrame.
+    
+    iSplitL "R0z".
+    by iExists r0_.
+
+    iSplitL "R1z".
+    by iExists r1_.
+
+    by iExists r0_'.
+    }
+
+    iSimpl.
+    iDestruct "HWPs" as "(HWP1 & HWP2)".
+    iSplitL "HWP1".
+    iSpecialize ("HWP1" with "[//]").
+    iIntros "_".
+    iApply (wp_mono with "HWP1").
+    intros k.
+    iStartProof.
+    iIntros "[? _]".
+    done.
+    iSplit; last done.
+    iIntros "Hprop".
+    iSpecialize ("HWP2" with "Hprop").
+    iApply (wp_mono with "HWP2").
+    intros k.
+    iStartProof.
+    iIntros "_".
+    done.
+
+    iIntros "interp".
+
+    unfold gen_vm_interp.
+    (* TODO: Open the provided invariant, prove pure prop *)
+    iExists ⊤.
+    iModIntro.
+    done.
+  Qed.
+  
 End Adequacy.
